Add more structure to Coq code, change LTT and PLTT names.
LTT is now CPS, that is, Complete Program Semantics
PLTT is now PPS, that is, Partial Program Semantics

Intermediate contains code regarding the intermediate
level (old LTT,PLTT etc), while Common contains the adapted
CompCert definitions for simulations, some auxiliary code (Util.v)
and global definitions (i.e. what is a program interface)

Intermediate/CPS_PPS.v
@@ -1,20 +1,19 @@
-Require Import Common.
-Require Import Events.
-Require Import Machine.
-Require Import LTT.
-Require Import PLTT.
-Require Import Smallstep.
-Require Import Behavior.
+Require Import Common.Definitions.
+Require Import Common.Util.
+Require Import Common.Events.
+Require Import Common.Smallstep.
+Require Import Common.Behavior.
+Require Import Intermediate.Machine.
+Require Import Intermediate.CPS.
+Require Import Intermediate.PPS.
 
 Require Import Coq.Logic.Classical.
 
-Module LTT_TO_PLTT.
+Import IntermediateMachine.
 
-Include AbstractMachine.
-
-Section SIMULATION.
-  Variable p : LTT.program.
-  Variable pp : PLTT.program.
+Section CPS_PPS_SIMULATION.
+  Variable p : CPS.program.
+  Variable pp : PPS.program.
   Variable split : list Component.id.
 
   (* the split is well-formed w.r.t. to the program interface *)
@@ -22,58 +21,58 @@ Section SIMULATION.
     forall C,
       In C split ->
     exists CI,
-      In CI (LTT.prog_interface p) /\ Component.name CI = C.
+      In CI (CPS.prog_interface p) /\ Component.name CI = C.
 
   (* the partial program is obtained by "splitting" the original
      program w.r.t. to split *)
   Hypothesis p_transfto_pp :
-    pp = PLTT.apply_split p split splitWF.
+    pp = PPS.apply_split p split splitWF.
 
   (* build the global environments *)
-  Let G := LTT.mkGlobalEnv (LTT.prog_interface p)
-                           (LTT.prog_entrypoints p).
-  Let G' := PLTT.mkGlobalEnv (LTT.prog_interface p)
-                             (LTT.prog_entrypoints p)
+  Let G := CPS.mkGlobalEnv (CPS.prog_interface p)
+                           (CPS.prog_entrypoints p).
+  Let G' := PPS.mkGlobalEnv (CPS.prog_interface p)
+                             (CPS.prog_entrypoints p)
                              split.
 
   Inductive match_states (split : list Component.id)
-    : LTT.state -> PLTT.partial_state -> Prop :=
+    : CPS.state -> PPS.partial_state -> Prop :=
   | program_control:
       forall C s ps mem pmem regs pc,
-        PLTT.is_program_component C split ->
-        ps = PLTT.to_partial_stack s split ->
-        PLTT.maps_match_on split mem pmem ->
+        PPS.is_program_component C split ->
+        ps = PPS.to_partial_stack s split ->
+        PPS.maps_match_on split mem pmem ->
         match_states split
                      (C, s, mem, regs, pc)
-                     (PLTT.PC (C, ps, pmem, regs, pc))
+                     (PPS.PC (C, ps, pmem, regs, pc))
 
   | context_control:
       forall C s ps mem pmem regs pc,
-        PLTT.is_context_component C split ->
-        ps = PLTT.to_partial_stack s split ->
-        PLTT.maps_match_on split mem pmem ->
+        PPS.is_context_component C split ->
+        ps = PPS.to_partial_stack s split ->
+        PPS.maps_match_on split mem pmem ->
         match_states split
                      (C, s, mem, regs, pc)
-                     (PLTT.CC (C, ps, pmem) PLTT.Normal)
+                     (PPS.CC (C, ps, pmem) PPS.Normal)
 
   | context_went_wrong:
       forall C s ps mem pmem regs pc,
-        PLTT.is_context_component C split ->
-        ps = PLTT.to_partial_stack s split ->
-        PLTT.maps_match_on split mem pmem ->
-        (forall s' t, ~ LTT.step G (C,s,mem,regs,pc) t s') ->
-        ~ LTT.final_state (C,s,mem,regs,pc) ->
+        PPS.is_context_component C split ->
+        ps = PPS.to_partial_stack s split ->
+        PPS.maps_match_on split mem pmem ->
+        (forall s' t, ~ CPS.step G (C,s,mem,regs,pc) t s') ->
+        ~ CPS.final_state (C,s,mem,regs,pc) ->
         match_states split
                      (C, s, mem, regs, pc)
-                     (PLTT.CC (C, ps, pmem) PLTT.WentWrong).
+                     (PPS.CC (C, ps, pmem) PPS.WentWrong).
 
   Hint Constructors match_states.
 
   Lemma initial_states_match:
     forall s,
-      LTT.initial_state p s ->
+      CPS.initial_state p s ->
     exists ps,
-      PLTT.initial_state pp ps /\ match_states split s ps.
+      PPS.initial_state pp ps /\ match_states split s ps.
   Proof.
     intros s Hs_init.
     rewrite p_transfto_pp.
@@ -82,62 +81,62 @@ Section SIMULATION.
     destruct Hs_init
       as [C_is_0 [empty_stack [empty_regs main_proc]]].
     destruct (Util.mem 0 split) eqn:Hcontrol.
-    - exists (PLTT.PC (0, [], mem, regs,
-                       EntryPoint.get 0 0 (LTT.genv_entrypoints G))).
+    - exists (PPS.PC (0, [], mem, regs,
+                       EntryPoint.get 0 0 (CPS.genv_entrypoints G))).
       split.
-      + unfold PLTT.initial_state.
+      + unfold PPS.initial_state.
         split; auto.
       + rewrite C_is_0, empty_stack, empty_regs, main_proc. simpl.
         apply program_control; auto.
-        * unfold PLTT.is_program_component.
+        * unfold PPS.is_program_component.
           apply Util.in_iff_mem_true. auto.
-    - exists (PLTT.CC (0, [], mem) PLTT.Normal).
+    - exists (PPS.CC (0, [], mem) PPS.Normal).
       split.
-      + unfold PLTT.initial_state.
+      + unfold PPS.initial_state.
         split; auto.
       + rewrite C_is_0, empty_stack, empty_regs, main_proc. simpl.
         apply context_control; auto.
-        * unfold PLTT.is_context_component.
+        * unfold PPS.is_context_component.
           apply Util.not_in_iff_mem_false. auto.
   Qed.
 
   Lemma final_states_match:
     forall s ps,
       match_states split s ps ->
-      LTT.final_state s ->
-      PLTT.final_state ps.
+      CPS.final_state s ->
+      PPS.final_state ps.
   Proof.
     intros s ps Hmatch_states Hs_final.
     destruct s
       as [[[[C d] mem] regs] pc] eqn:Hstate_s.
-    unfold LTT.final_state in Hs_final.
+    unfold CPS.final_state in Hs_final.
     inversion Hmatch_states; subst;
-      unfold PLTT.final_state; auto.
+      unfold PPS.final_state; auto.
     - exfalso. apply H9. auto.
   Qed.
 
   Lemma lockstep_simulation:
     forall s t s',
-      LTT.step G s t s' ->
+      CPS.step G s t s' ->
       forall ps,
         match_states split s ps ->
       exists ps',
-        PLTT.step G' ps t ps' /\ match_states split s' ps'.
+        PPS.step G' ps t ps' /\ match_states split s' ps'.
   Proof.
     intros s t s'.
     intros Hstep ps Hmatch_states.
 
     (* extract the currently executing component memory *)
-    destruct (LTT.step_implies_memory_existence G s t s' Hstep)
+    destruct (CPS.step_implies_memory_existence G s t s' Hstep)
       as [Cmem HCmem].
 
     (* useful facts *)
-    pose (LTT.prog_entrypoints p) as E.
-    pose (LTT.prog_entrypoints_wf p) as EWF.
+    pose (CPS.prog_entrypoints p) as E.
+    pose (CPS.prog_entrypoints_wf p) as EWF.
     assert (HG_unfolded:
               G = {|
-                LTT.genv_interfaces := LTT.genv_interfaces G;
-                LTT.genv_entrypoints := LTT.genv_entrypoints G
+                CPS.genv_interfaces := CPS.genv_interfaces G;
+                CPS.genv_entrypoints := CPS.genv_entrypoints G
               |}). {
       destruct G. simpl. auto.
     } rewrite HG_unfolded in Hstep.
@@ -159,13 +158,13 @@ Section SIMULATION.
 
         (* context epsilon steps (except store) *)
         try (eexists; split;
-             [ apply PLTT.Context_Epsilon
+             [ apply PPS.Context_Epsilon
              | apply context_control; auto
              ]);
 
         (* program epsilon steps (except store) *)
         try (eexists; split;
-             [ eapply PLTT.Program_Epsilon;
+             [ eapply PPS.Program_Epsilon;
                [ apply HCmem
                | apply HCmem
                | eauto
@@ -180,7 +179,7 @@ Section SIMULATION.
         try (exfalso; eapply Hno_step; eauto).
 
     (* program store *)
-    - exists (PLTT.PC (C, PLTT.to_partial_stack d split,
+    - exists (PPS.PC (C, PPS.to_partial_stack d split,
                        Memory.set pmem C
                                   (Register.get r1 regs)
                                   (Register.get r2 regs),
@@ -191,13 +190,13 @@ Section SIMULATION.
                     (Register.get r1 regs)
                     (Register.get r2 regs) Cmem)
           as updated_Cmem.
-        eapply PLTT.Program_Epsilon with
+        eapply PPS.Program_Epsilon with
             (s:=d) (cmem:=Cmem)
             (cmem':=updated_Cmem)
             (wmem':=M.add C updated_Cmem mem).
         * apply HCmem.
         * apply M.add_1. reflexivity.
-        * unfold PLTT.maps_match_on.
+        * unfold PPS.maps_match_on.
           intros. split; intro; eassumption.
         * unfold Memory.set in Hstep.
           rewrite (M.find_1 HCmem) in Hstep.
@@ -213,7 +212,7 @@ Section SIMULATION.
           ** assumption.
       (* states match *)
       + apply program_control; auto.
-        * apply PLTT.update_related_memories with
+        * apply PPS.update_related_memories with
               (C:=C) (mem1:=mem) (mem2:=pmem)
               (addr:=Register.get r1 regs)
               (val:=Register.get r2 regs);
@@ -223,7 +222,7 @@ Section SIMULATION.
     - destruct (in_dec Nat.eq_dec C' split) as [ HC'origin | ? ];
         eexists; split.
       (* internal call - step *)
-      + apply PLTT.Program_Internal_Call; auto.
+      + apply PPS.Program_Internal_Call; auto.
       (* internal call - states match *)
       + destruct (splitWF C' HC'origin)
           as [C'I [C'I_in_I C'I_name_is_C']].
@@ -239,7 +238,7 @@ Section SIMULATION.
         * eauto.
         * auto.
       (* external call - step *)
-      + apply PLTT.Program_External_Call; auto.
+      + apply PPS.Program_External_Call; auto.
       (* external call - states match *)
       + apply context_control; auto.
         * simpl.
@@ -252,14 +251,14 @@ Section SIMULATION.
         as [ HC'origin | HC'origin ];
         eexists; split.
       (* internal return - step *)
-      + apply PLTT.Program_Internal_Return; auto.
+      + apply PPS.Program_Internal_Return; auto.
         * simpl.
           apply Util.in_iff_mem_true in HC'origin.
           rewrite HC'origin. reflexivity.
       (* internal return - states match *)
       + eauto.
       (* external return - step *)
-      + apply PLTT.Program_External_Return; auto.
+      + apply PPS.Program_External_Return; auto.
         * simpl.
           apply Util.not_in_iff_mem_false in HC'origin.
           rewrite HC'origin. reflexivity.
@@ -267,7 +266,7 @@ Section SIMULATION.
       + eauto.
 
     (* context store - states match *)
-    - unfold PLTT.maps_match_on.
+    - unfold PPS.maps_match_on.
       intros C' C'mem HC'origin.
       split.
       + intro HC'map.
@@ -289,7 +288,7 @@ Section SIMULATION.
           rewrite <- HeqCC' in HC'origin. apply HC'origin. }
         unfold Memory.set.
         destruct (M.find (elt:=list nat) C mem) eqn:HCfind.
-        * assert (HC'mem: PLTT.M.MapsTo C' C'mem mem).
+        * assert (HC'mem: M.MapsTo C' C'mem mem).
           { apply Hmem; assumption. }
           eapply M.add_2; assumption.
         * apply Hmem; auto.
@@ -298,9 +297,9 @@ Section SIMULATION.
     - destruct (in_dec Nat.eq_dec C' split) as [ HC'origin | ? ];
         eexists; split.
       (* external call - step *)
-      + apply PLTT.Context_External_Call;
+      + apply PPS.Context_External_Call;
           try assumption.
-        * apply PLTT.push_by_context_preserves_partial_stack; eauto.
+        * apply PPS.push_by_context_preserves_partial_stack; eauto.
       (* external call - states match *)
       + destruct (splitWF C' HC'origin)
           as [CI [CI_in_I CI_name_is_C']].
@@ -312,9 +311,9 @@ Section SIMULATION.
         * eauto.
         * assumption.
       (* internal call - step *)
-      + apply PLTT.Context_Internal_Call;
+      + apply PPS.Context_Internal_Call;
           try assumption.
-        * apply PLTT.push_by_context_preserves_partial_stack; eauto.
+        * apply PPS.push_by_context_preserves_partial_stack; eauto.
       (* internal call - states match *)
       + eauto.
 
@@ -322,21 +321,21 @@ Section SIMULATION.
     - destruct (in_dec Nat.eq_dec C' split) as [HC'origin | ?];
         eexists; split.
       (* external return - step*)
-      + apply PLTT.Context_External_Return; auto.
+      + apply PPS.Context_External_Return; auto.
         * simpl. apply Util.in_iff_mem_true in HC'origin.
           rewrite HC'origin.
           reflexivity.
       (* external return - states match *)
       + eauto.
       (* internal return - step *)
-      + apply PLTT.Context_Internal_Return; auto.
-        * apply PLTT.push_by_context_preserves_partial_stack; auto.
+      + apply PPS.Context_Internal_Return; auto.
+        * apply PPS.push_by_context_preserves_partial_stack; auto.
       (* internal return - states match *)
       + eauto.
   Qed.
 
-  Theorem forward_simulation_between_LTT_and_PLTT:
-    forward_simulation (LTT.semantics p) (PLTT.semantics pp).
+  Theorem forward_simulation_between_CPS_and_PPS:
+    forward_simulation (CPS.semantics p) (PPS.semantics pp).
   Proof.
     apply forward_simulation_step with (match_states split).
     - apply initial_states_match.
@@ -345,52 +344,41 @@ Section SIMULATION.
       apply lockstep_simulation.
   Defined.
 
-  Corollary not_wrong_behavior_preservation:
-    forall beh,
-      not_wrong beh ->
-      program_behaves (LTT.semantics p) beh ->
-      program_behaves (PLTT.semantics pp) beh.
-  Proof.
-    intros beh Hnotwrong Hprogbeh.
-    eapply forward_simulation_same_safe_behavior; eauto.
-    apply forward_simulation_between_LTT_and_PLTT.
-  Qed.
-
-  (* We can prove something stronger, that is, PLTT 
+  (* We can prove something stronger, that is, PPS 
      preserves exactly all behaviors. *)
 
   (* IDEA:
-     when LTT goes wrong we might be in two cases:
-     - the program is executing, which means that PLTT
+     when CPS goes wrong we might be in two cases:
+     - the program is executing, which means that PPS
        must be stuck as well
      - the context is executing, which means that the
        last step of our simulation must go into a 
        WentWrong state
      by proving this two lemmas, we should be able to
      show that the trace produced when going wrong
-     is exactly the same we observed in LTT.
+     is exactly the same we observed in CPS.
    *)
 
   Lemma nonfinal_preservation_for_program:
     forall s pstate,
-      match_states split s (PLTT.PC pstate) ->
-      ~ LTT.final_state s ->
-      ~ PLTT.final_state (PLTT.PC pstate).
+      match_states split s (PPS.PC pstate) ->
+      ~ CPS.final_state s ->
+      ~ PPS.final_state (PPS.PC pstate).
   Proof.
     intros s pstate Hmatch_states Hnot_final.
-    unfold not, PLTT.final_state.
+    unfold not, PPS.final_state.
     destruct pstate as [[[[C d] mem] regs] pc].
     destruct s as [[[[C' d'] mem'] regs'] pc'].
     intro Hhalt.
-    apply Hnot_final. unfold LTT.final_state.
+    apply Hnot_final. unfold CPS.final_state.
     inversion Hmatch_states; subst. auto.
   Qed.
 
   Lemma nostep_preservation_for_program:
     forall s pstate,
-      match_states split s (PLTT.PC pstate) ->
-      (forall t s', ~ LTT.step G s t s') -> 
-      (forall t ps', ~ PLTT.step G' (PLTT.PC pstate) t ps'). 
+      match_states split s (PPS.PC pstate) ->
+      (forall t s', ~ CPS.step G s t s') -> 
+      (forall t ps', ~ PPS.step G' (PPS.PC pstate) t ps'). 
   Proof.
     intros s pstate Hmatch_states Hnostep.
     intros t ps'. unfold not. intro contra.
@@ -398,38 +386,38 @@ Section SIMULATION.
     inversion contra; subst;
       (* epsilon steps *)
       try (match goal with
-             Hmaps_match : PLTT.maps_match_on split ?MEM ?PMEM,
-             HCwmem : PLTT.M.MapsTo ?C ?CMEM ?WMEM,
-             HCwmem' : PLTT.M.MapsTo ?C ?CMEM' ?WMEM',
-             HLTTstep : LTT.step ?ENV1 ?S E0 ?S',
-             HCpmem : PLTT.M.MapsTo ?C ?CMEM ?PMEM,
-             Hcontra : PLTT.step ?ENV2 ?PS E0 ?PS'
+             Hmaps_match : PPS.maps_match_on split ?MEM ?PMEM,
+             HCwmem : M.MapsTo ?C ?CMEM ?WMEM,
+             HCwmem' : M.MapsTo ?C ?CMEM' ?WMEM',
+             HCPSstep : CPS.step ?ENV1 ?S E0 ?S',
+             HCpmem : M.MapsTo ?C ?CMEM ?PMEM,
+             Hcontra : PPS.step ?ENV2 ?PS E0 ?PS'
              |- _ => apply Hmaps_match in HCpmem; eauto;
-                     destruct (LTT.epsilon_step_weakening
-                                 (PLTT.genv_interfaces G') E
+                     destruct (CPS.epsilon_step_weakening
+                                 (PPS.genv_interfaces G') E
                                  C s wmem wmem' cmem cmem'
-                                 regs regs' pc pc' HCwmem HCwmem' HLTTstep
-                                 (PLTT.genv_entrypoints G')
+                                 regs regs' pc pc' HCwmem HCwmem' HCPSstep
+                                 (PPS.genv_entrypoints G')
                                  s0 mem HCpmem);
                      eapply Hnostep; eauto
            end);
       (* Calls *)
       try (match goal with
-             Hcontra : PLTT.executing (PLTT.Call ?C2 ?P) ?C ?MEM ?PC
-             |- _ => eapply Hnostep; eapply LTT.Call; eauto
+             Hcontra : executing (Call ?C2 ?P) ?C ?MEM ?PC
+             |- _ => eapply Hnostep; eapply CPS.Call; eauto
            end);
       (* Returns *)
       try (match goal with
-             Hpartial_stack : PLTT.to_partial_stack ?STACK split = ?PSTACK,
-             Hcontra : PLTT.executing PLTT.Return ?C ?MEM ?PC
+             Hpartial_stack : PPS.to_partial_stack ?STACK split = ?PSTACK,
+             Hcontra : executing Return ?C ?MEM ?PC
              |- _ => destruct s0; inversion Hpartial_stack;
                      destruct p0; subst;
-                     unfold PLTT.to_partial_stack in Hpartial_stack;
+                     unfold PPS.to_partial_stack in Hpartial_stack;
                      simpl in Hpartial_stack;
                      inversion Hpartial_stack;
                      destruct (Util.mem i split);
                      inversion H1; inversion H2; subst;
-                     eapply Hnostep; eapply LTT.Return; eauto
+                     eapply Hnostep; eapply CPS.Return; eauto
            end).
   Qed.
 
@@ -467,15 +455,15 @@ Section SIMULATION.
     end.
 
   Definition s_match_states :=
-    sim_rel forward_simulation_between_LTT_and_PLTT.
+    sim_rel forward_simulation_between_CPS_and_PPS.
 
   Definition s_props :=
-    sim_props forward_simulation_between_LTT_and_PLTT.
+    sim_props forward_simulation_between_CPS_and_PPS.
 
   Lemma generic_match_implies_specific_match:
     forall i s pstate,
-      s_match_states i s (PLTT.PC pstate) ->
-      SIMULATION.match_states split s (PLTT.PC pstate).
+      s_match_states i s (PPS.PC pstate) ->
+      CPS_PPS_SIMULATION.match_states split s (PPS.PC pstate).
   Proof.
     intros i s pstate Hmatch_states.
     destruct Hmatch_states; auto.
@@ -483,28 +471,28 @@ Section SIMULATION.
 
   Lemma goes_wrong_preservation:
     forall i s ps t s',
-      Star (LTT.semantics p) s t s' ->
-      Nostep (LTT.semantics p) s' ->
-      ~final_state (LTT.semantics p) s' ->
+      Star (CPS.semantics p) s t s' ->
+      Nostep (CPS.semantics p) s' ->
+      ~final_state (CPS.semantics p) s' ->
       s_match_states i s ps ->
     exists ps',
-      Star (PLTT.semantics pp) ps t ps' /\
-      Nostep (PLTT.semantics pp) ps' /\
-      ~final_state (PLTT.semantics pp) ps'.
+      Star (PPS.semantics pp) ps t ps' /\
+      Nostep (PPS.semantics pp) ps' /\
+      ~final_state (PPS.semantics pp) ps'.
   Proof.
     intros i s ps t s'.
-    intros HLTT_star HLTT_nostep HLTT_nofinal.
+    intros HCPS_star HCPS_nostep HCPS_nofinal.
     intros Hs_match_states.
     destruct (simulation_star
-                s_props HLTT_star i ps Hs_match_states)
-      as [i' [ps' [HPLTT_star Hs_match_states']]].
+                s_props HCPS_star i ps Hs_match_states)
+      as [i' [ps' [HPPS_star Hs_match_states']]].
     destruct ps' as [pstate | cstate exec_state].
     (* the program got stuck *)
-    - exists (PLTT.PC pstate). split; auto. split.
+    - exists (PPS.PC pstate). split; auto. split.
       (* we cannot step anymore *)
       + simpl. unfold nostep.
         rewrite p_transfto_pp.
-        unfold PLTT.apply_split. simpl.
+        unfold PPS.apply_split. simpl.
         eapply nostep_preservation_for_program;
           eauto.
         apply (generic_match_implies_specific_match i');
@@ -515,17 +503,17 @@ Section SIMULATION.
         apply (generic_match_implies_specific_match i');
           auto.
     (* the context got stuck *)
-    - exists (PLTT.CC cstate PLTT.WentWrong).
+    - exists (PPS.CC cstate PPS.WentWrong).
       split.
       (* we prove that there exists a star execution *)
       * destruct exec_state.
         (* the execution is in a normal state, hence we make
            an ulterior step to go in a WentWrong state *)
         ** apply star_right with
-               t (PLTT.CC cstate PLTT.Normal) E0.
-           *** apply HPLTT_star.
+               t (PPS.CC cstate PPS.Normal) E0.
+           *** apply HPPS_star.
            *** destruct cstate. destruct p0.
-               apply PLTT.Context_GoesWrong.
+               apply PPS.Context_GoesWrong.
            *** symmetry. apply E0_right.
         (* the execution is already in a WentWrong state*)
         ** auto.
@@ -537,10 +525,10 @@ Section SIMULATION.
         (* WentWrong is not final *)
         ** unfold not. intro.
            enough (Hnot_final:
-                     ~ PLTT.final_state
-                       (PLTT.CC cstate PLTT.WentWrong)).
+                     ~ PPS.final_state
+                       (PPS.CC cstate PPS.WentWrong)).
            apply Hnot_final; auto.
-           unfold not, PLTT.final_state.
+           unfold not, PPS.final_state.
            destruct cstate as [[C d] mem].
            intro contra. inversion contra.
   Qed.
@@ -548,8 +536,8 @@ Section SIMULATION.
   Theorem state_goes_wrong_preservation:
     forall i s ps t,
       s_match_states i s ps ->
-      state_behaves (LTT.semantics p) s (Goes_wrong t) ->
-      state_behaves (PLTT.semantics pp) ps (Goes_wrong t).
+      state_behaves (CPS.semantics p) s (Goes_wrong t) ->
+      state_behaves (PPS.semantics pp) ps (Goes_wrong t).
   Proof.
     intros i s ps t Hmatch_states Hstatebeh.
     inversion Hstatebeh.
@@ -561,8 +549,8 @@ Section SIMULATION.
 
   Theorem wrong_behavior_preservation:
     forall t,
-      program_behaves (LTT.semantics p) (Goes_wrong t) ->
-      program_behaves (PLTT.semantics pp) (Goes_wrong t).
+      program_behaves (CPS.semantics p) (Goes_wrong t) ->
+      program_behaves (PPS.semantics pp) (Goes_wrong t).
   Proof.
     intros t Hprogbeh.
     inversion Hprogbeh as [ s beh Hs_init Hstatebeh
@@ -577,20 +565,20 @@ Section SIMULATION.
     (* goes intially wrong *)
     - assert (Hgoingwrong_state:
                 exists ps,
-                  ps = (PLTT.CC (0%nat, [],
+                  ps = (PPS.CC (0%nat, [],
                                  @M.empty (list nat))
-                                PLTT.WentWrong) /\
-                  Nostep (PLTT.semantics pp) ps /\
-                  PLTT.initial_state pp ps /\
-                  ~PLTT.final_state ps). {
-        exists (PLTT.CC (0%nat, [], @M.empty (list nat))
-                        PLTT.WentWrong).
+                                PPS.WentWrong) /\
+                  Nostep (PPS.semantics pp) ps /\
+                  PPS.initial_state pp ps /\
+                  ~PPS.final_state ps). {
+        exists (PPS.CC (0%nat, [], @M.empty (list nat))
+                        PPS.WentWrong).
         split; auto.
         split.
         - unfold nostep. intros.
           unfold not. intro contra. inversion contra.
-        - unfold PLTT.initial_state. split; auto.
-          unfold PLTT.final_state.
+        - unfold PPS.initial_state. split; auto.
+          unfold PPS.final_state.
           unfold not. intro contra. inversion contra.
       }
       destruct Hgoingwrong_state
@@ -598,8 +586,8 @@ Section SIMULATION.
                              [Hps_init Hps_notfinal]]]].
       apply program_runs with ps; eauto. subst.
       apply state_goes_wrong with
-          (PLTT.CC (0%nat, [], M.empty (list nat))
-                   PLTT.WentWrong).
+          (PPS.CC (0%nat, [], M.empty (list nat))
+                   PPS.WentWrong).
       apply star_refl; auto.
       unfold nostep. intros t ps' contra.
       inversion contra.
@@ -609,191 +597,28 @@ Section SIMULATION.
 
   Corollary strong_behavior_preservation:
     forall beh,
-      program_behaves (LTT.semantics p) beh ->
-      program_behaves (PLTT.semantics pp) beh.
+      program_behaves (CPS.semantics p) beh ->
+      program_behaves (PPS.semantics pp) beh.
   Proof.
     intros beh Hprogbeh.
     destruct beh.
     - eapply forward_simulation_same_safe_behavior; eauto.
-      apply forward_simulation_between_LTT_and_PLTT.
+      apply forward_simulation_between_CPS_and_PPS.
       simpl. reflexivity.
     - eapply forward_simulation_same_safe_behavior; eauto.
-      apply forward_simulation_between_LTT_and_PLTT.
+      apply forward_simulation_between_CPS_and_PPS.
       simpl. reflexivity.
     - eapply forward_simulation_same_safe_behavior; eauto.
-      apply forward_simulation_between_LTT_and_PLTT.
+      apply forward_simulation_between_CPS_and_PPS.
       simpl. reflexivity.
-    - destruct forward_simulation_between_LTT_and_PLTT.
+    - destruct forward_simulation_between_CPS_and_PPS.
       apply wrong_behavior_preservation; auto.
   Qed.
 
-  (* OLD ATTEMPTS (the last one is interesting because
-     is generic and doesn't rely on the specific instance
-     of forward simulation that we built)
-  
-  (* 1st ATTEMPT (with SECTION à la CompCert) *)
+  (* OLD ATTEMPT (it is interesting because is generic and
+     doesn't rely on the specific instance of forward
+     simulation that we built)
 
-  Section FORWARD_SIMULATION.
-    Context index order match_states
-            (S: fsim_properties
-                  (LTT.semantics p) (PLTT.semantics pp)
-                  index order match_states).
-
-    Lemma generic_match_implies_specific_match:
-      forall i s pstate,
-        match_states i s (PLTT.PC pstate) ->
-        SIMULATION.match_states split s (PLTT.PC pstate).
-    Proof.
-      intros i s pstate Hmatch_states.
-    Admitted.
-
-    Lemma goes_wrong_preservation:
-      forall i s ps t s',
-        Star (LTT.semantics p) s t s' ->
-        Nostep (LTT.semantics p) s' ->
-        ~final_state (LTT.semantics p) s' ->
-        match_states i s ps ->
-      exists ps',
-        Star (PLTT.semantics pp) ps t ps' /\
-        Nostep (PLTT.semantics pp) ps' /\
-        ~final_state (PLTT.semantics pp) ps'.
-    Proof.
-      intros i s ps t s'.
-      intros HLTT_star HLTT_nostep HLTT_nofinal.
-      intros Hmatch_states.
-      destruct (simulation_star
-                  S HLTT_star i ps Hmatch_states)
-        as [i' [ps' [HPLTT_star Hmatch_states']]].
-      destruct ps' as [pstate | cstate exec_state].
-      (* the program got stuck *)
-      - exists (PLTT.PC pstate). split; auto. split.
-        (* we cannot step anymore *)
-        + simpl. unfold nostep.
-          rewrite p_transfto_pp.
-          unfold PLTT.apply_split. simpl.
-          eapply nostep_preservation_for_program;
-            eauto.
-          apply (generic_match_implies_specific_match i');
-            auto.
-        (* we are not in a final state *)
-        + apply nonfinal_preservation_for_program with s';
-            eauto.
-          apply (generic_match_implies_specific_match i');
-            auto.
-      (* the context got stuck *)
-      - exists (PLTT.CC cstate PLTT.WentWrong).
-        split.
-        * destruct exec_state.
-          ** apply star_right with
-                 t (PLTT.CC cstate PLTT.Normal) E0.
-             *** apply HPLTT_star.
-             *** destruct cstate. destruct p0.
-                 apply PLTT.Context_GoesWrong.
-             *** symmetry. apply E0_right.
-          ** auto.
-        * split.
-          (* WentWrong doesn't step *)
-          ** unfold nostep. intros.
-             unfold not. intro contra. inversion contra.
-          (* WentWrong is not final *)
-          ** unfold not. intro.
-             enough (Hnot_final:
-                       ~ PLTT.final_state
-                         (PLTT.CC cstate PLTT.WentWrong)).
-             apply Hnot_final; auto.
-             unfold not, PLTT.final_state.
-             destruct cstate. destruct p0.
-             intro contra. inversion contra.
-    Qed.
-
-    Theorem state_goes_wrong_preservation:
-      forall i s ps t,
-        match_states i s ps ->
-        state_behaves (LTT.semantics p) s (Goes_wrong t) ->
-        state_behaves (PLTT.semantics pp) ps (Goes_wrong t).
-    Proof.
-      intros i s ps t Hmatch_states Hstatebeh.
-      inversion Hstatebeh.
-      destruct (goes_wrong_preservation
-             i s ps t s' H0 H1 H2 Hmatch_states)
-        as [ps' [Hps_star [Hps_nostep Hps_notfinal]]].
-      eapply state_goes_wrong; eauto.
-    Qed.
-
-    Theorem wrong_behavior_preservation:
-      forall t,
-        program_behaves (LTT.semantics p) (Goes_wrong t) ->
-        program_behaves (PLTT.semantics pp) (Goes_wrong t).
-    Proof.
-      intros t Hprogbeh.
-      inversion Hprogbeh as [ s beh Hs_init Hstatebeh
-                            | Hnot_init ].
-      (* goes wrong with non-empty trace *)
-      - (* initial states *)
-        destruct (fsim_match_initial_states S s Hs_init)
-          as [i [ps [Hps_init Hmatch_states]]].
-        (* simulation *)
-        eapply program_runs; eauto.
-        apply state_goes_wrong_preservation with i s; auto.
-      (* goes intially wrong *)
-      - assert (Hgoingwrong_state:
-          exists ps,
-            ps = (PLTT.CC (0%nat, [],
-                           @M.empty (list nat))
-                          PLTT.WentWrong) /\
-            Nostep (PLTT.semantics pp) ps /\
-            PLTT.initial_state pp ps /\
-            ~PLTT.final_state ps). {
-          exists (PLTT.CC (0%nat, [], @M.empty (list nat))
-                          PLTT.WentWrong).
-          split; auto.
-          split.
-          - unfold nostep. intros.
-            unfold not. intro contra. inversion contra.
-          - unfold PLTT.initial_state. split; auto.
-            unfold PLTT.final_state.
-            unfold not. intro contra. inversion contra.
-        }
-        destruct Hgoingwrong_state
-          as [ps [Hps_state [Hps_nostep
-                               [Hps_init Hps_notfinal]]]].
-        apply program_runs with ps; eauto. subst.
-        apply state_goes_wrong with
-            (PLTT.CC (0%nat, [], M.empty (list nat))
-                     PLTT.WentWrong).
-        apply star_refl; auto.
-        unfold nostep. intros t ps' contra.
-        inversion contra.
-        unfold not. intro contra.
-        apply Hps_notfinal. auto.
-    Qed.
-  End FORWARD_SIMULATION.
-
-  Corollary strong_behavior_preservation:
-    forall beh,
-      program_behaves (LTT.semantics p) beh ->
-      program_behaves (PLTT.semantics pp) beh.
-  Proof.
-    intros beh Hprogbeh.
-    destruct beh.
-    - eapply forward_simulation_same_safe_behavior; eauto.
-      apply forward_simulation_between_LTT_and_PLTT.
-      simpl. reflexivity.
-    - eapply forward_simulation_same_safe_behavior; eauto.
-      apply forward_simulation_between_LTT_and_PLTT.
-      simpl. reflexivity.
-    - eapply forward_simulation_same_safe_behavior; eauto.
-      apply forward_simulation_between_LTT_and_PLTT.
-      simpl. reflexivity.
-    - destruct forward_simulation_between_LTT_and_PLTT.
-      apply wrong_behavior_preservation with
-          index order match_states0; auto.
-  Qed.
-
-  (* STUCK! We cannot prove the two lemmas about
-     generic nostep and nonfinal preservation! *)
-
-  (* 2nd ATTEMPT *)
   (* Let's try with a stronger notion of simulation *)
 
   Record fsim_properties'
@@ -940,5 +765,4 @@ Section SIMULATION.
   End FORWARD_SIMULATION_2.
   (* Stuck! Even here we have problems with the same lemmas! *)
 *)
-End SIMULATION.
-End LTT_TO_PLTT.
+End CPS_PPS_SIMULATION.
