Intermediate/PPS.v
@@ -1,0 +1,353 @@
+Require Import Common.Definitions.
+Require Import Common.Util.
+Require Import Common.Events.
+Require Import Common.Smallstep.
+Require Import Intermediate.Machine.
+Require Import Intermediate.CPS.
+
+Module PPS.
+  Import IntermediateMachine.
+
+  Record program := {
+    prog_interface : Program.interface;
+    prog_memory : Memory.data;
+    prog_entrypoints : EntryPoint.data;
+    prog_split : list Component.id;
+    prog_entrypoints_wf :
+      forall CI C,
+        In CI prog_interface ->
+        Component.name CI = C ->
+        In C prog_split ->
+        M.In C prog_entrypoints /\
+        exists addrs, M.MapsTo C addrs prog_entrypoints;
+    prog_split_wf :
+      forall C,
+        In C prog_split ->
+        exists CI, In CI prog_interface /\ Component.name CI = C
+  }.
+
+  Definition stack := list (Component.id * option Memory.address).
+
+  Definition program_state : Type :=
+    Component.id * stack * Memory.data * Register.data * Memory.address.
+  Definition context_state : Type :=
+    Component.id * stack * Memory.data.
+
+  Inductive exec_state : Type :=
+  | Normal
+  | WentWrong.
+
+  Inductive partial_state : Type :=
+  | PC : program_state -> partial_state
+  | CC : context_state -> exec_state -> partial_state.
+
+  Definition to_partial_frame pc frame : Component.id * option Memory.address :=
+    match frame with (C,i) =>
+      if Util.mem C pc then (C, Some i) else (C, None)
+    end.
+
+  Definition to_partial_stack (s : CPS.stack) (pc : list Component.id) :=
+    map (to_partial_frame pc) s.
+
+  Lemma push_by_prog_preserves_partial_stack :
+    forall s ps pc C i,
+      Util.mem C pc = true ->
+      to_partial_stack s pc = ps ->
+      to_partial_stack ((C,i)::s) pc = (C,Some i) :: ps.
+  Proof.
+    intros s ps pc C i Hprogturn H.
+    simpl. rewrite Hprogturn. rewrite H. reflexivity.
+  Qed.
+
+  Lemma push_by_context_preserves_partial_stack :
+    forall s ps pc C i,
+      ~ (In C pc) ->
+      to_partial_stack s pc = ps ->
+      to_partial_stack ((C,i)::s) pc = (C,None) :: ps.
+  Proof.
+    intros s ps pc C i Hprogturn Hpstack.
+    simpl. apply Util.not_in_iff_mem_false in Hprogturn.
+    rewrite Hprogturn. rewrite Hpstack. reflexivity.
+  Qed.
+
+  Record global_env := mkGlobalEnv {
+    genv_interfaces : Program.interface;
+    genv_entrypoints : EntryPoint.data;
+    genv_split : list Component.id;
+  }.
+
+  Definition initial_state_for
+             (p : program) (split : list Component.id) : partial_state :=
+    let mem := prog_memory p in
+    let E := prog_entrypoints p in
+    let split := prog_split p in
+    if Util.mem 0 split then
+      PC (0, [], mem, Register.empty, EntryPoint.get 0 0 E)
+    else
+      CC (0, [], mem) Normal.
+
+  Definition initial_state p (s : partial_state) : Prop :=
+    match s with
+    | PC (C, d, mem, regs, pc) =>
+      C = 0 /\ d = [] /\ regs = Register.empty /\
+      pc = EntryPoint.get 0 0 (prog_entrypoints p)
+    | CC (C, d, mem) state =>
+      C = 0 /\ d = []
+    end.
+
+  Definition final_state (s : partial_state) : Prop :=
+    match s with
+    | PC (C, d, mem, regs, pc) =>
+      executing Halt C mem pc
+    | CC (C, d, mem) state =>
+      state = Normal
+    end.
+
+  Definition is_program_component C (prog_comps : list Component.id) :=
+    In C prog_comps.
+  Definition is_context_component C (prog_comps : list Component.id) :=
+    ~ (In C prog_comps).
+
+  Definition maps_match_on {T : Type} split (map map' : M.t T) :=
+    forall C Cmap,
+      PPS.is_program_component C split ->
+      (M.MapsTo C Cmap map <-> M.MapsTo C Cmap map').
+
+  Reserved Notation "G |-PPS s1 '=>[' t ']' s2" (at level 40).
+
+  Inductive step (G : global_env)
+    : partial_state -> trace -> partial_state -> Prop :=
+  | Program_Epsilon:
+      forall E C s ps
+             mem mem' wmem wmem' cmem cmem'
+             regs regs' pc pc',
+        M.MapsTo C cmem wmem ->
+        M.MapsTo C cmem' wmem' ->
+        maps_match_on (genv_split G) E (genv_entrypoints G) ->
+        let G' := CPS.mkGlobalEnv (genv_interfaces G) E in
+        CPS.step G' (C,s,wmem,regs,pc) E0 (C,s,wmem',regs',pc') ->
+        M.MapsTo C cmem mem ->
+        M.MapsTo C cmem' mem' ->
+        G |-PPS (PC (C,ps,mem,regs,pc)) =>[E0] (PC (C,ps,mem',regs',pc'))
+
+  | Program_Internal_Call:
+      forall mem C pc regs d d' C' P,
+        executing (Call C' P) C mem pc ->
+        C' <> C ->
+        call_is_public_and_exists (genv_interfaces G) C' P ->
+        call_is_in_imports (genv_interfaces G) C C' P ->
+        is_program_component C' (genv_split G) ->
+        d' = (C,Some (pc+1)) :: d ->
+        let t := [ECall C P (Register.get Register.R_COM regs) C'] in
+        G |-PPS (PC (C,d,mem,regs,pc)) =>[t]
+                (PC (C',d',mem,regs,EntryPoint.get C' P (genv_entrypoints G)))
+
+  | Program_Internal_Return:
+      forall mem C C' pc pc' d d' regs,
+        executing Return C mem pc ->
+        C' <> C ->
+        is_program_component C' (genv_split G) ->
+        d = (C',Some pc') :: d' ->
+        let t := [ERet C (Register.get Register.R_COM regs) C'] in
+        G |-PPS (PC (C,d,mem,regs,pc)) =>[t] (PC (C',d',mem,regs,pc'))
+
+  | Program_External_Call:
+      forall mem C pc regs d d' C' P,
+        executing (Call C' P) C mem pc ->
+        C' <> C ->
+        call_is_public_and_exists (genv_interfaces G) C' P ->
+        call_is_in_imports (genv_interfaces G) C C' P ->
+        is_context_component C' (genv_split G) ->
+        d' = (C,Some (pc+1)) :: d ->
+        let t := [ECall C P (Register.get Register.R_COM regs) C'] in
+        G |-PPS (PC (C,d,mem,regs,pc)) =>[t] (CC (C',d',mem) Normal)
+
+  | Program_External_Return:
+      forall mem C C' pc d d' regs,
+        executing Return C mem pc ->
+        C' <> C ->
+        is_context_component C' (genv_split G) ->
+        d = (C',None) :: d' ->
+        let t := [ERet C (Register.get Register.R_COM regs) C'] in
+        G |-PPS (PC (C,d,mem,regs,pc)) =>[t] (CC (C',d',mem) Normal)
+
+  | Context_Epsilon:
+      forall mem C d,
+        G |-PPS (CC (C,d,mem) Normal) =>[E0] (CC (C,d,mem) Normal)
+
+  | Context_GoesWrong:
+      forall mem C d,
+        G |-PPS (CC (C,d,mem) Normal) =>[E0] (CC (C,d,mem) WentWrong)
+
+  | Context_Internal_Call:
+      forall mem C d d' C' P call_arg,
+        C' <> C ->
+        call_is_public_and_exists (genv_interfaces G) C' P ->
+        call_is_in_imports (genv_interfaces G) C C' P ->
+        is_context_component C' (genv_split G) ->
+        d' = (C,None) :: d ->
+        let t := [ECall C P call_arg C'] in
+        G |-PPS (CC (C,d,mem) Normal) =>[t] (CC (C',d',mem) Normal)
+
+  | Context_Internal_Return:
+      forall mem C C' d d' return_val,
+        C' <> C ->
+        is_context_component C' (genv_split G) ->
+        d = (C',None) :: d' ->
+        let t := [ERet C return_val C'] in
+        G |-PPS (CC (C,d,mem) Normal) =>[t] (CC (C',d',mem) Normal)
+
+  | Context_External_Call:
+      forall mem C regs d d' C' P,
+        C' <> C ->
+        call_is_public_and_exists (genv_interfaces G) C' P ->
+        call_is_in_imports (genv_interfaces G) C C' P ->
+        is_program_component C' (genv_split G) ->
+        d' = (C,None) :: d ->
+        let t := [ECall C P (Register.get Register.R_COM regs) C'] in
+        G |-PPS (CC (C,d,mem) Normal) =>[t]
+                (PC (C',d',mem,regs,EntryPoint.get C' P (genv_entrypoints G)))
+
+  | Context_External_Return:
+      forall mem C C' pc' d d' regs,
+        d = (C',Some pc') :: d' ->
+        is_program_component C' (genv_split G) ->
+        let t := [ERet C (Register.get Register.R_COM regs) C'] in
+        G |-PPS (CC (C,d,mem) Normal) =>[t] (PC (C',d',mem,regs,pc'))
+
+  where "G |-PPS s1 '=>[' t ']' s2" := (step G s1 t s2).
+
+  Lemma maps_match_on_reflexive :
+    forall T split (map : M.t T),
+      maps_match_on split map map.
+  Proof.
+    split; intros; auto.
+  Qed.
+
+  Lemma maps_match_on_symmetric :
+    forall T split (map1 map2 : M.t T),
+      maps_match_on split map1 map2 ->
+      maps_match_on split map2 map1.
+  Proof.
+    intros ? split map1 map2 Hmaps_match.
+    split; intro; apply Hmaps_match; auto.
+  Qed.
+
+  Hint Resolve maps_match_on_reflexive.
+  Hint Resolve maps_match_on_symmetric.
+
+  Lemma update_related_memories_generic :
+    forall split mem1 mem2 C Cmem C' addr val,
+      maps_match_on split mem1 mem2 ->
+      is_program_component C split ->
+      M.MapsTo C Cmem (Memory.set mem1 C' addr val) ->
+      M.MapsTo C Cmem (Memory.set mem2 C' addr val).
+  Proof.
+    intros split mem1 mem2 C Cmem C' addr val.
+    intros Hmems_match HCorigin HCmem.
+    unfold Memory.set.
+    unfold Memory.set in HCmem.
+    destruct (C =? C') eqn:HeqCC'.
+    + apply beq_nat_true in HeqCC'. subst.
+      destruct (M.find (elt:=list nat) C' mem2) eqn:Hfind.
+      * apply M.find_2 in Hfind. apply Hmems_match in Hfind.
+        ** rewrite (M.find_1 Hfind) in HCmem.
+           apply M.find_2.
+           apply M.find_1 in HCmem.
+           rewrite <- HCmem.
+           rewrite F.add_eq_o, F.add_eq_o;
+             reflexivity.
+        ** assumption.
+      * apply Hmems_match.
+        ** assumption.
+        ** assert (M.find (elt:=list nat) C' mem1 = None).
+           { destruct (M.find (elt:=list nat) C' mem1) eqn:Hfind'.
+             *** exfalso.
+                 apply F.not_find_in_iff in Hfind. apply Hfind.
+                 exists l. apply Hmems_match.
+                 **** assumption.
+                 **** apply M.find_2. assumption.
+             *** reflexivity. }
+           rewrite H in HCmem. assumption.
+    + apply beq_nat_false in HeqCC'.
+      destruct (M.find (elt:=list nat) C' mem2) eqn:Hfind.
+      * apply M.add_2.
+        ** unfold not. intro. apply HeqCC'. symmetry. apply H.
+        ** apply Hmems_match.
+           *** assumption.
+           *** destruct (M.find (elt:=list nat) C' mem1) eqn:Hfind'.
+               **** eapply M.add_3.
+                    ***** intro. apply HeqCC'. symmetry. apply H.
+                    ***** apply HCmem.
+               **** assumption.
+      * apply Hmems_match.
+        ** assumption.
+        ** destruct (M.find (elt:=list nat) C' mem1) eqn:Hfind'.
+           *** eapply M.add_3.
+               **** intro. apply HeqCC'. symmetry. apply H.
+               **** apply HCmem.
+           *** assumption.
+  Qed.
+
+  Lemma update_related_memories :
+    forall split mem1 mem1' mem2 mem2' C addr val,
+      maps_match_on split mem1 mem2 ->
+      mem1' = Memory.set mem1 C addr val ->
+      mem2' = Memory.set mem2 C addr val ->
+      maps_match_on split mem1' mem2'.
+  Proof.
+    intros split mem1 mem1' mem2 mem2' C addr val.
+    intros Hmems_match Hmem1' Hmem2'.
+    unfold PPS.maps_match_on.
+    intros C0 C0mem HC0_origin.
+    split;
+      intro HC0map;
+      [ rewrite Hmem2';
+        rewrite Hmem1' in HC0map;
+        apply update_related_memories_generic with
+            (split:=split) (mem1:=mem1) (mem2:=mem2)
+      | rewrite Hmem1';
+        rewrite Hmem2' in HC0map;
+        apply update_related_memories_generic with
+            (split:=split) (mem1:=mem2) (mem2:=mem1) ];
+      auto.
+  Qed.
+
+  Section SEMANTICS.
+    Variable p : program.
+
+    Definition semantics :=
+      @Semantics_gen partial_state global_env
+                     step
+                     (initial_state p)
+                     final_state
+                     (mkGlobalEnv (prog_interface p)
+                                  (prog_entrypoints p)
+                                  (prog_split p)).
+  End SEMANTICS.
+
+  (* if entrypoints are well-formed, then they remain
+     well-formed even if we consider only the ones relative
+     to the components in the split *)
+  Lemma entrypoints_exist_wrt_split split :
+    forall p CI C,
+      In CI (CPS.prog_interface p) ->
+      Component.name CI = C ->
+      In C split ->
+      M.In C (CPS.prog_entrypoints p) /\
+      exists addrs, M.MapsTo C addrs (CPS.prog_entrypoints p).
+  Proof.
+    intros p CI C.
+    intros HCI_in_I HCI_name_is_C HC_in_split.
+    apply (CPS.prog_entrypoints_wf p) with CI; assumption.
+  Qed.
+
+  Definition apply_split (p : CPS.program) split splitWF :=
+    {| prog_interface := CPS.prog_interface p;
+       prog_memory := CPS.prog_memory p;
+       prog_entrypoints := CPS.prog_entrypoints p;
+       prog_split := split;
+       prog_entrypoints_wf :=
+         entrypoints_exist_wrt_split split p;
+       prog_split_wf := splitWF |}.
+End PPS.
